doc: document AIG up to current status

LeanSAT/Heap.lean
@@ -12,56 +12,140 @@ theorem Array.push_get_old (as : Array α) (a : α) (h : i < as.size) : (as.push
 theorem Array.push_get_size (as : Array α) (a : α) : (as.push a)[as.size] = a := by
   simp [Array.push_get]
 
-
+/--
+A circuit node declaration. These are not recursive but instead contain indices into an `Env`.
+-/
 inductive Decl where
-| const (b : Bool)
-| atom (idx : Nat)
-| gate (x y : Nat) (xpol ypol : Bool)
-deriving BEq, Hashable, Repr
+  /--
+  A node with a constant output value.
+  -/
+  | const (b : Bool)
+  /--
+  An input node to the circuit.
+  -/
+  | atom (idx : Nat)
+  /--
+  An AIG gate with configurable input nodes and polarity.
+  -/
+  | gate (x y : Nat) (xpol ypol : Bool)
+  deriving BEq, Hashable, Repr
 
+/--
+A `Cache` is valid with respect to a list of declarations iff:
+Whenever `cache.find? decl` returns an index into `xs : Array Decl`, `xs[index] = decl`.
+This predicate limits a `HashMap Decl Nat` to this behavior.
+-/
 inductive Cache.WF : Array Decl → HashMap Decl Nat → Prop where
-| empty : Cache.WF decls HashMap.empty
-| push_id (h : Cache.WF decls cache) : Cache.WF (decls.push decl) cache
-| push_cache (h : Cache.WF decls cache) : Cache.WF (decls.push decl) (cache.insert decl decls.size)
+  /--
+  An empty `Cache` is valid for any `Array Decl` as it never has a hit.
+  -/
+  | empty : Cache.WF decls HashMap.empty
+  /--
+  Given a `cache`, valid with respect to some `decls`, we can extend the `decls` without
+  extending the cache and remain valid.
+  -/
+  | push_id (h : Cache.WF decls cache) : Cache.WF (decls.push decl) cache
+  /--
+  Given a `cache`, valid with respect to some `decls`, we can extend the `decls`
+  and the `cache` at the same time with the same values and remaind valid.
+  -/
+  | push_cache (h : Cache.WF decls cache) : Cache.WF (decls.push decl) (cache.insert decl decls.size)
 
+/--
+A cache that is valid with respect to some `Array Decl`.
+-/
 def Cache (decls : Array Decl) := { map : HashMap Decl Nat // Cache.WF decls map }
 
+/--
+Create an empty `Cache`, valid with respect to any `Array Decl`.
+-/
 def Cache.empty (decls : Array Decl) : Cache decl := ⟨HashMap.empty, WF.empty⟩
 
+@[inherit_doc Cache.WF.push_id]
 def Cache.noUpdate (cache : Cache decls) : Cache (decls.push decl) :=
   ⟨cache.val, Cache.WF.push_id cache.property⟩
 
+@[inherit_doc Cache.WF.push_cache]
 def Cache.insert (cache : Cache decls) (decl : Decl) : Cache (decls.push decl) :=
   ⟨cache.val.insert decl decls.size, Cache.WF.push_cache cache.property⟩
 
+/--
+Lookup a `decl` in a `cache`. 
+
+If this returns `some i`, `Cache.find?_poperty` can be used to demonstrate: `decls[i] = decl`.
+-/
 def Cache.find? (cache : Cache decls) (decl : Decl) : Option Nat :=
   cache.val.find? decl
 
--- TODO: This is probably provable by building a better cache API
+/--
+This axiom states that all indices, found in a `Cache` that is valid with respect to some `decls`,
+are within bounds of `decls`.
+-/
 axiom Cache.find?_bounds {decls : Array Decl} {idx : Nat} (c : Cache decls) (decl : Decl)
     (h : c.find? decl = some idx) : idx < decls.size
 
+/--
+This axiom states that if `Cache.find? decl` returns `some i`, `decls[i] = decl`, holds.
+-/
 axiom Cache.find?_property {decls : Array Decl} {idx : Nat} (c : Cache decls) (decl : Decl)
     (h : c.find? decl = some idx) : decls[idx]'(Cache.find?_bounds c decl h) = decl
 
+/--
+An `Array Decl` is a Direct Acyclic Graph (DAG) if this holds.
+-/
 def IsDag (decls : Array Decl) : Prop := ∀ i lhs rhs lpol rpol (h : i < decls.size), decls[i] = .gate lhs rhs lpol rpol → lhs < i ∧ rhs < i
+
+/--
+The empty array is a DAG.
+-/
 theorem IsDag.empty : IsDag #[] := by
   intro i lhs rhs lpol rpol h
   simp only [Array.size_toArray, List.length_nil] at h
   omega
 
+/--
+An And Inverter Graph (AIG) together with a cache for subterm sharing.
+-/
 structure Env where
+  /--
+  The circuit itself as an `Array Decl` whose members have indices into said array.
+  -/
   decls : Array Decl
+  /--
+  The `Decl` cache, valid with respect to `decls`.
+  -/
   cache : Cache decls
+  /--
+  In order to be a valid AIG, `decls` must form a DAG.
+  -/
   inv : IsDag decls
 
+/--
+An `Env` with an empty AIG and cache.
+-/
 def Env.empty : Env := { decls := #[], cache := Cache.empty #[], inv := IsDag.empty }
 
+/--
+An entrypoint into an `Env`. This can be used to evaluate a circuit, starting at a certain node,
+with `Env.denote` or to construct bigger circuits
+-/
 structure Env.Entrypoint where
+  /--
+  The AIG that we are in.
+  -/
   env : Env
+  /--
+  The AIG node at which to begin evaluation.
+  -/
   start : Nat
+  /--
+  The AIG node must be within bounds.
+  -/
   inv : start < env.decls.size
 
+/--
+Evaluate an `Env.Entrypoint` using some assignment for atoms.
+-/
 def Env.denote (entry : Env.Entrypoint) (assign : List Bool) : Bool :=
   go entry.start entry.env.decls assign entry.inv entry.env.inv
 where
@@ -75,6 +159,9 @@ where
       let rval := go rhs decls assign (by omega) h2
       xor lval lpol && xor rval rpol
 
+/--
+Running `Env.denote.go` on a node that is within bounds of `decls` is equivalent to running it a bigger `decls` array.
+-/
 theorem Env.denote.go_lt_push (x : Nat) (decls : Array Decl) (h1 : x < decls.size) {h2} {h3} (inv : IsDag decls) :
     (denote.go x decls assign h1 h2) = (denote.go x (decls.push decl) assign (by simp; omega) h3) := by
   unfold denote.go
@@ -108,6 +195,10 @@ theorem Env.denote.go_lt_push (x : Nat) (decls : Array Decl) (h1 : x < decls.siz
           assumption
         . rfl
 
+/--
+Build an AIG gate in `env`. Note that his version is only meant for proving,
+for production purposes use `Env.mkGateCached` and equality theorems to this one.
+-/
 def Env.mkGate (lhs rhs : Nat) (lpol rpol : Bool) (env : Env) (hl : lhs < env.decls.size) 
     (hr : rhs < env.decls.size) : Env.Entrypoint :=
   let g := env.decls.size
@@ -121,10 +212,17 @@ def Env.mkGate (lhs rhs : Nat) (lpol rpol : Bool) (env : Env) (hl : lhs < env.de
     . injections; omega
   ⟨{ env with decls, inv, cache }, g, by simp [g, decls]⟩
 
+/--
+`Env.mkGate` never shrinks the underlying AIG.
+-/
 theorem Env.mkGate_le_size (lhs rhs : Nat) (lpol rpol : Bool) (env : Env) hl hr
     : env.decls.size ≤ (env.mkGate lhs rhs lpol rpol hl hr).env.decls.size := by
   simp_arith [mkGate]
 
+/--
+Reusing an `Env.Entrypoint` to build an additional gate will never invalidate the entry node of
+the original entrypoint.
+-/
 theorem Env.lt_mkGate_size (e1 : Env.Entrypoint) (lhs rhs : Nat) (lpol rpol : Bool) hl hr
     : e1.start < (e1.env.mkGate lhs rhs lpol rpol hl hr).env.decls.size := by
   have h1 := e1.inv
@@ -132,6 +230,10 @@ theorem Env.lt_mkGate_size (e1 : Env.Entrypoint) (lhs rhs : Nat) (lpol rpol : Bo
     Env.mkGate_le_size _ _ _ _ _ _ _
   omega
 
+/--
+A version of `Env.mkGate` that uses the subterm cache in `Env`. This version is meant for
+programmming, for proving purposes use `Env.mkGate` and equality theorems to this one.
+-/
 def Env.mkGateCached (lhs rhs : Nat) (lpol rpol : Bool) (env : Env) (hl : lhs < env.decls.size)
     (hr : rhs < env.decls.size) : Env.Entrypoint :=
   let decl := .gate lhs rhs lpol rpol
@@ -151,6 +253,9 @@ def Env.mkGateCached (lhs rhs : Nat) (lpol rpol : Bool) (env : Env) (hl : lhs < 
       . injections; omega
     ⟨{ env with decls, inv, cache }, g, by simp [g, decls]⟩
 
+/--
+The central equality theorem between `mkGateCached` and `mkGate`.
+-/
 theorem Env.mkGateCached_eval_eq_mkGate_eval (lhs rhs : Nat) (lpol rpol : Bool) (env : Env) (hl : lhs < env.decls.size)
     (hr : rhs < env.decls.size) : denote (env.mkGateCached lhs rhs lpol rpol hl hr) assign = denote (env.mkGate lhs rhs lpol rpol hl hr) assign := by
   simp only [mkGate, mkGateCached]
@@ -179,6 +284,10 @@ theorem Env.mkGateCached_eval_eq_mkGate_eval (lhs rhs : Nat) (lpol rpol : Bool) 
           . rfl
   . simp [denote]
 
+/--
+Add a new input node to the AIG in `env`. Note that his version is only meant for proving,
+for production purposes use `Env.mkAtomCached` and equality theorems to this one.
+-/
 def Env.mkAtom (n : Nat) (env : Env) : Env.Entrypoint :=
   let g := env.decls.size
   let decls := env.decls.push (.atom n)
@@ -192,10 +301,17 @@ def Env.mkAtom (n : Nat) (env : Env) : Env.Entrypoint :=
     . contradiction
   ⟨{ decls, inv, cache }, g, by simp [g, decls]⟩
 
+/--
+`Env.mkAtom` never shrinks the underlying AIG.
+-/
 theorem Env.mkAtom_le_size (env : Env) (var : Nat)
     : env.decls.size ≤ (env.mkAtom var).env.decls.size := by
   simp_arith [mkAtom]
 
+/--
+A version of `Env.mkAtom` that uses the subterm cache in `Env`. This version is meant for
+programmming, for proving purposes use `Env.mkAtom` and equality theorems to this one.
+-/
 def Env.mkAtomCached (n : Nat) (env : Env) : Env.Entrypoint :=
   let decl := .atom n
   match h:env.cache.find? decl with
@@ -214,6 +330,9 @@ def Env.mkAtomCached (n : Nat) (env : Env) : Env.Entrypoint :=
       . contradiction
   ⟨{ decls, inv, cache }, g, by simp [g, decls]⟩
 
+/--
+The central equality theorem between `mkAtomCached` and `mkAtom`.
+-/
 theorem Env.mkAtomCached_eval_eq_mkAtom_eval (var : Nat) (env : Env)
     : denote (env.mkAtomCached var) assign = denote (env.mkAtom var) assign := by
   simp only [mkAtom, mkAtomCached]
@@ -236,6 +355,10 @@ theorem Env.mkAtomCached_eval_eq_mkAtom_eval (var : Nat) (env : Env)
     . next heq2 => rw [h1] at heq2; injections
   . simp [denote]
 
+/--
+Build an constant node in `env`. Note that his version is only meant for proving,
+for production purposes use `Env.mkConstCached` and equality theorems to this one.
+-/
 def Env.mkConst (val : Bool) (env : Env) : Env.Entrypoint :=
   let g := env.decls.size
   let decls := env.decls.push (.const val)
@@ -249,16 +372,27 @@ def Env.mkConst (val : Bool) (env : Env) : Env.Entrypoint :=
     . contradiction
   ⟨{ decls, inv, cache }, g, by simp [g, decls]⟩
 
+/--
+`Env.mkConst` never shrinks the underlying AIG.
+-/
 theorem Env.mkConst_le_size (env : Env) (val : Bool)
     : env.decls.size ≤ (env.mkConst val).env.decls.size := by
   simp_arith [mkConst]
 
+/--
+Reusing an `Env.Entrypoint` to build an additional constant will never invalidate the entry node of
+the original entrypoint.
+-/
 theorem Env.lt_mkConst_size (e1 : Env.Entrypoint) : e1.start < (e1.env.mkConst val).env.decls.size := by
   have h1 := e1.inv
   have h2 : e1.env.decls.size ≤ (e1.env.mkConst val).env.decls.size :=
     Env.mkConst_le_size _ _
   omega
 
+/--
+A version of `Env.mkConst` that uses the subterm cache in `Env`. This version is meant for
+programmming, for proving purposes use `Env.mkGate` and equality theorems to this one.
+-/
 def Env.mkConstCached (val : Bool) (env : Env) : Env.Entrypoint :=
   let decl := .const val
   match h:env.cache.find? decl with
@@ -277,6 +411,9 @@ def Env.mkConstCached (val : Bool) (env : Env) : Env.Entrypoint :=
       . contradiction
   ⟨{ decls, inv, cache }, g, by simp [g, decls]⟩
 
+/--
+The central equality theorem between `mkConstCached` and `mkConst`.
+-/
 theorem Env.mkConstCached_eval_eq_mkConst_eval (val : Bool) (env : Env)
     : denote (env.mkConstCached val) assign = denote (env.mkConst val) assign := by
   simp only [mkConst, mkConstCached]
@@ -300,10 +437,21 @@ theorem Env.mkConstCached_eval_eq_mkConst_eval (val : Bool) (env : Env)
     . next heq2 => rw [h1] at heq2; injections
   . simp [denote]
 
--- TODO: implement version of this with cached functions and prove equivalent
+-- TODO: implement cached version of this with cached functions and prove equivalent
+/--
+Turn a `BoolExprNat` into an AIG + entrypoint. Note that this version is only meant
+for proving purposes. For programming use `Env.ofBoolExprNatCached` and equality theorems.
+-/
 def Env.ofBoolExprNat (expr : BoolExprNat) : Env.Entrypoint :=
-  go expr Env.empty
+  go expr Env.empty |>.val
 where
+  /-
+  This function contains a series of `have` statements that fulfill no obvious purpose.
+  They are used to prove the `env.decls.size ≤ entry.env.decls.size` invariant of the return
+  value with the final omega call in each case. This invariant is necessary as we recursively
+  call this function multiple times so we need to guarantee that no recursive call ever shrinks
+  the AIG in order to be allowed to use the generated AIG nodes.
+  -/
   go (expr : BoolExprNat) (env : Env) : { entry : Env.Entrypoint // env.decls.size ≤ entry.env.decls.size } :=
     match expr with
     | .literal var => ⟨env.mkAtom var, (by apply Env.mkAtom_le_size)⟩
